ristretto255/proofs/fstar/extraction/Ristretto255.Scalar.fst
@@ -45,6 +45,22 @@ val impl_6': Core_models.Cmp.t_Eq t_Scalar
 unfold
 let impl_6 = impl_6'
 
+/// Generate a random scalar using the provided RNG.
+assume
+val impl_Scalar__random':
+    #v_R: Type0 ->
+    {| i0: Rand_core.t_RngCore v_R |} ->
+    {| i1: Rand_core.t_CryptoRng v_R |} ->
+    rng: v_R
+  -> (v_R & t_Scalar)
+
+unfold
+let impl_Scalar__random
+      (#v_R: Type0)
+      (#[FStar.Tactics.Typeclasses.tcresolve ()] i0: Rand_core.t_RngCore v_R)
+      (#[FStar.Tactics.Typeclasses.tcresolve ()] i1: Rand_core.t_CryptoRng v_R)
+     = impl_Scalar__random' #v_R #i0 #i1
+
 /// Serialize this scalar to a 32-byte little-endian array.
 let impl_Scalar__to_bytes (self: t_Scalar) : t_Array u8 (mk_usize 32) = self._0
 
@@ -72,302 +88,69 @@ let impl_Scalar52__ZERO: t_Scalar52 =
   <:
   t_Scalar52
 
-let impl_Scalar52__from_bytes (bytes: t_Array u8 (mk_usize 32)) : t_Scalar52 =
-  let words:t_Array u64 (mk_usize 4) = Rust_primitives.Hax.repeat (mk_u64 0) (mk_usize 4) in
-  let words:t_Array u64 (mk_usize 4) =
-    Rust_primitives.Hax.Folds.fold_range (mk_usize 0)
-      (mk_usize 4)
-      (fun words temp_1_ ->
-          let words:t_Array u64 (mk_usize 4) = words in
-          let _:usize = temp_1_ in
-          true)
-      words
-      (fun words i ->
-          let words:t_Array u64 (mk_usize 4) = words in
-          let i:usize = i in
-          Rust_primitives.Hax.Folds.fold_range (mk_usize 0)
-            (mk_usize 8)
-            (fun words temp_1_ ->
-                let words:t_Array u64 (mk_usize 4) = words in
-                let _:usize = temp_1_ in
-                true)
-            words
-            (fun words j ->
-                let words:t_Array u64 (mk_usize 4) = words in
-                let j:usize = j in
-                Rust_primitives.Hax.Monomorphized_update_at.update_at_usize words
-                  i
-                  ((words.[ i ] <: u64) |.
-                    ((cast (bytes.[ (i *! mk_usize 8 <: usize) +! j <: usize ] <: u8) <: u64) <<!
-                      (j *! mk_usize 8 <: usize)
-                      <:
-                      u64)
-                    <:
-                    u64)
-                <:
-                t_Array u64 (mk_usize 4))
-          <:
-          t_Array u64 (mk_usize 4))
-  in
-  let mask:u64 = (mk_u64 1 <<! mk_i32 52 <: u64) -! mk_u64 1 in
-  let top_mask:u64 = (mk_u64 1 <<! mk_i32 48 <: u64) -! mk_u64 1 in
-  Scalar52
-  (let list =
-      [
-        (words.[ mk_usize 0 ] <: u64) &. mask;
-        (((words.[ mk_usize 0 ] <: u64) >>! mk_i32 52 <: u64) |.
-          ((words.[ mk_usize 1 ] <: u64) <<! mk_i32 12 <: u64)
-          <:
-          u64) &.
-        mask;
-        (((words.[ mk_usize 1 ] <: u64) >>! mk_i32 40 <: u64) |.
-          ((words.[ mk_usize 2 ] <: u64) <<! mk_i32 24 <: u64)
-          <:
-          u64) &.
-        mask;
-        (((words.[ mk_usize 2 ] <: u64) >>! mk_i32 28 <: u64) |.
-          ((words.[ mk_usize 3 ] <: u64) <<! mk_i32 36 <: u64)
-          <:
-          u64) &.
-        mask;
-        ((words.[ mk_usize 3 ] <: u64) >>! mk_i32 16 <: u64) &. top_mask
-      ]
-    in
-    FStar.Pervasives.assert_norm (Prims.eq2 (List.Tot.length list) 5);
-    Rust_primitives.Hax.array_of_list 5 list)
-  <:
-  t_Scalar52
+assume
+val impl_Scalar52__from_bytes': bytes: t_Array u8 (mk_usize 32) -> t_Scalar52
 
-let impl_Scalar52__to_bytes (self: t_Scalar52) : t_Array u8 (mk_usize 32) =
-  let s:t_Array u8 (mk_usize 32) = Rust_primitives.Hax.repeat (mk_u8 0) (mk_usize 32) in
-  let s:t_Array u8 (mk_usize 32) =
-    Rust_primitives.Hax.Monomorphized_update_at.update_at_usize s
-      (mk_usize 0)
-      (cast ((self._0.[ mk_usize 0 ] <: u64) >>! mk_i32 0 <: u64) <: u8)
-  in
-  let s:t_Array u8 (mk_usize 32) =
-    Rust_primitives.Hax.Monomorphized_update_at.update_at_usize s
-      (mk_usize 1)
-      (cast ((self._0.[ mk_usize 0 ] <: u64) >>! mk_i32 8 <: u64) <: u8)
-  in
-  let s:t_Array u8 (mk_usize 32) =
-    Rust_primitives.Hax.Monomorphized_update_at.update_at_usize s
-      (mk_usize 2)
-      (cast ((self._0.[ mk_usize 0 ] <: u64) >>! mk_i32 16 <: u64) <: u8)
-  in
-  let s:t_Array u8 (mk_usize 32) =
-    Rust_primitives.Hax.Monomorphized_update_at.update_at_usize s
-      (mk_usize 3)
-      (cast ((self._0.[ mk_usize 0 ] <: u64) >>! mk_i32 24 <: u64) <: u8)
-  in
-  let s:t_Array u8 (mk_usize 32) =
-    Rust_primitives.Hax.Monomorphized_update_at.update_at_usize s
-      (mk_usize 4)
-      (cast ((self._0.[ mk_usize 0 ] <: u64) >>! mk_i32 32 <: u64) <: u8)
-  in
-  let s:t_Array u8 (mk_usize 32) =
-    Rust_primitives.Hax.Monomorphized_update_at.update_at_usize s
-      (mk_usize 5)
-      (cast ((self._0.[ mk_usize 0 ] <: u64) >>! mk_i32 40 <: u64) <: u8)
-  in
-  let s:t_Array u8 (mk_usize 32) =
-    Rust_primitives.Hax.Monomorphized_update_at.update_at_usize s
-      (mk_usize 6)
-      (cast (((self._0.[ mk_usize 0 ] <: u64) >>! mk_i32 48 <: u64) |.
-            ((self._0.[ mk_usize 1 ] <: u64) <<! mk_i32 4 <: u64)
-            <:
-            u64)
-        <:
-        u8)
-  in
-  let s:t_Array u8 (mk_usize 32) =
-    Rust_primitives.Hax.Monomorphized_update_at.update_at_usize s
-      (mk_usize 7)
-      (cast ((self._0.[ mk_usize 1 ] <: u64) >>! mk_i32 4 <: u64) <: u8)
-  in
-  let s:t_Array u8 (mk_usize 32) =
-    Rust_primitives.Hax.Monomorphized_update_at.update_at_usize s
-      (mk_usize 8)
-      (cast ((self._0.[ mk_usize 1 ] <: u64) >>! mk_i32 12 <: u64) <: u8)
-  in
-  let s:t_Array u8 (mk_usize 32) =
-    Rust_primitives.Hax.Monomorphized_update_at.update_at_usize s
-      (mk_usize 9)
-      (cast ((self._0.[ mk_usize 1 ] <: u64) >>! mk_i32 20 <: u64) <: u8)
-  in
-  let s:t_Array u8 (mk_usize 32) =
-    Rust_primitives.Hax.Monomorphized_update_at.update_at_usize s
-      (mk_usize 10)
-      (cast ((self._0.[ mk_usize 1 ] <: u64) >>! mk_i32 28 <: u64) <: u8)
-  in
-  let s:t_Array u8 (mk_usize 32) =
-    Rust_primitives.Hax.Monomorphized_update_at.update_at_usize s
-      (mk_usize 11)
-      (cast ((self._0.[ mk_usize 1 ] <: u64) >>! mk_i32 36 <: u64) <: u8)
-  in
-  let s:t_Array u8 (mk_usize 32) =
-    Rust_primitives.Hax.Monomorphized_update_at.update_at_usize s
-      (mk_usize 12)
-      (cast ((self._0.[ mk_usize 1 ] <: u64) >>! mk_i32 44 <: u64) <: u8)
-  in
-  let s:t_Array u8 (mk_usize 32) =
-    Rust_primitives.Hax.Monomorphized_update_at.update_at_usize s
-      (mk_usize 13)
-      (cast ((self._0.[ mk_usize 2 ] <: u64) >>! mk_i32 0 <: u64) <: u8)
-  in
-  let s:t_Array u8 (mk_usize 32) =
-    Rust_primitives.Hax.Monomorphized_update_at.update_at_usize s
-      (mk_usize 14)
-      (cast ((self._0.[ mk_usize 2 ] <: u64) >>! mk_i32 8 <: u64) <: u8)
-  in
-  let s:t_Array u8 (mk_usize 32) =
-    Rust_primitives.Hax.Monomorphized_update_at.update_at_usize s
-      (mk_usize 15)
-      (cast ((self._0.[ mk_usize 2 ] <: u64) >>! mk_i32 16 <: u64) <: u8)
-  in
-  let s:t_Array u8 (mk_usize 32) =
-    Rust_primitives.Hax.Monomorphized_update_at.update_at_usize s
-      (mk_usize 16)
-      (cast ((self._0.[ mk_usize 2 ] <: u64) >>! mk_i32 24 <: u64) <: u8)
-  in
-  let s:t_Array u8 (mk_usize 32) =
-    Rust_primitives.Hax.Monomorphized_update_at.update_at_usize s
-      (mk_usize 17)
-      (cast ((self._0.[ mk_usize 2 ] <: u64) >>! mk_i32 32 <: u64) <: u8)
-  in
-  let s:t_Array u8 (mk_usize 32) =
-    Rust_primitives.Hax.Monomorphized_update_at.update_at_usize s
-      (mk_usize 18)
-      (cast ((self._0.[ mk_usize 2 ] <: u64) >>! mk_i32 40 <: u64) <: u8)
-  in
-  let s:t_Array u8 (mk_usize 32) =
-    Rust_primitives.Hax.Monomorphized_update_at.update_at_usize s
-      (mk_usize 19)
-      (cast (((self._0.[ mk_usize 2 ] <: u64) >>! mk_i32 48 <: u64) |.
-            ((self._0.[ mk_usize 3 ] <: u64) <<! mk_i32 4 <: u64)
-            <:
-            u64)
-        <:
-        u8)
-  in
-  let s:t_Array u8 (mk_usize 32) =
-    Rust_primitives.Hax.Monomorphized_update_at.update_at_usize s
-      (mk_usize 20)
-      (cast ((self._0.[ mk_usize 3 ] <: u64) >>! mk_i32 4 <: u64) <: u8)
-  in
-  let s:t_Array u8 (mk_usize 32) =
-    Rust_primitives.Hax.Monomorphized_update_at.update_at_usize s
-      (mk_usize 21)
-      (cast ((self._0.[ mk_usize 3 ] <: u64) >>! mk_i32 12 <: u64) <: u8)
-  in
-  let s:t_Array u8 (mk_usize 32) =
-    Rust_primitives.Hax.Monomorphized_update_at.update_at_usize s
-      (mk_usize 22)
-      (cast ((self._0.[ mk_usize 3 ] <: u64) >>! mk_i32 20 <: u64) <: u8)
-  in
-  let s:t_Array u8 (mk_usize 32) =
-    Rust_primitives.Hax.Monomorphized_update_at.update_at_usize s
-      (mk_usize 23)
-      (cast ((self._0.[ mk_usize 3 ] <: u64) >>! mk_i32 28 <: u64) <: u8)
-  in
-  let s:t_Array u8 (mk_usize 32) =
-    Rust_primitives.Hax.Monomorphized_update_at.update_at_usize s
-      (mk_usize 24)
-      (cast ((self._0.[ mk_usize 3 ] <: u64) >>! mk_i32 36 <: u64) <: u8)
-  in
-  let s:t_Array u8 (mk_usize 32) =
-    Rust_primitives.Hax.Monomorphized_update_at.update_at_usize s
-      (mk_usize 25)
-      (cast ((self._0.[ mk_usize 3 ] <: u64) >>! mk_i32 44 <: u64) <: u8)
-  in
-  let s:t_Array u8 (mk_usize 32) =
-    Rust_primitives.Hax.Monomorphized_update_at.update_at_usize s
-      (mk_usize 26)
-      (cast ((self._0.[ mk_usize 4 ] <: u64) >>! mk_i32 0 <: u64) <: u8)
-  in
-  let s:t_Array u8 (mk_usize 32) =
-    Rust_primitives.Hax.Monomorphized_update_at.update_at_usize s
-      (mk_usize 27)
-      (cast ((self._0.[ mk_usize 4 ] <: u64) >>! mk_i32 8 <: u64) <: u8)
-  in
-  let s:t_Array u8 (mk_usize 32) =
-    Rust_primitives.Hax.Monomorphized_update_at.update_at_usize s
-      (mk_usize 28)
-      (cast ((self._0.[ mk_usize 4 ] <: u64) >>! mk_i32 16 <: u64) <: u8)
-  in
-  let s:t_Array u8 (mk_usize 32) =
-    Rust_primitives.Hax.Monomorphized_update_at.update_at_usize s
-      (mk_usize 29)
-      (cast ((self._0.[ mk_usize 4 ] <: u64) >>! mk_i32 24 <: u64) <: u8)
-  in
-  let s:t_Array u8 (mk_usize 32) =
-    Rust_primitives.Hax.Monomorphized_update_at.update_at_usize s
-      (mk_usize 30)
-      (cast ((self._0.[ mk_usize 4 ] <: u64) >>! mk_i32 32 <: u64) <: u8)
-  in
-  let s:t_Array u8 (mk_usize 32) =
-    Rust_primitives.Hax.Monomorphized_update_at.update_at_usize s
-      (mk_usize 31)
-      (cast ((self._0.[ mk_usize 4 ] <: u64) >>! mk_i32 40 <: u64) <: u8)
-  in
-  s
+unfold
+let impl_Scalar52__from_bytes = impl_Scalar52__from_bytes'
 
-let impl_Scalar52__mul_internal (a b: t_Scalar52) : t_Array u128 (mk_usize 9) =
-  let a:t_Array u64 (mk_usize 5) = a._0 in
-  let b:t_Array u64 (mk_usize 5) = b._0 in
-  let list =
-    [
-      m (a.[ mk_usize 0 ] <: u64) (b.[ mk_usize 0 ] <: u64);
-      (m (a.[ mk_usize 0 ] <: u64) (b.[ mk_usize 1 ] <: u64) <: u128) +!
-      (m (a.[ mk_usize 1 ] <: u64) (b.[ mk_usize 0 ] <: u64) <: u128);
-      ((m (a.[ mk_usize 0 ] <: u64) (b.[ mk_usize 2 ] <: u64) <: u128) +!
-        (m (a.[ mk_usize 1 ] <: u64) (b.[ mk_usize 1 ] <: u64) <: u128)
-        <:
-        u128) +!
-      (m (a.[ mk_usize 2 ] <: u64) (b.[ mk_usize 0 ] <: u64) <: u128);
-      (((m (a.[ mk_usize 0 ] <: u64) (b.[ mk_usize 3 ] <: u64) <: u128) +!
-          (m (a.[ mk_usize 1 ] <: u64) (b.[ mk_usize 2 ] <: u64) <: u128)
-          <:
-          u128) +!
-        (m (a.[ mk_usize 2 ] <: u64) (b.[ mk_usize 1 ] <: u64) <: u128)
-        <:
-        u128) +!
-      (m (a.[ mk_usize 3 ] <: u64) (b.[ mk_usize 0 ] <: u64) <: u128);
-      ((((m (a.[ mk_usize 0 ] <: u64) (b.[ mk_usize 4 ] <: u64) <: u128) +!
-            (m (a.[ mk_usize 1 ] <: u64) (b.[ mk_usize 3 ] <: u64) <: u128)
-            <:
-            u128) +!
-          (m (a.[ mk_usize 2 ] <: u64) (b.[ mk_usize 2 ] <: u64) <: u128)
-          <:
-          u128) +!
-        (m (a.[ mk_usize 3 ] <: u64) (b.[ mk_usize 1 ] <: u64) <: u128)
-        <:
-        u128) +!
-      (m (a.[ mk_usize 4 ] <: u64) (b.[ mk_usize 0 ] <: u64) <: u128);
-      (((m (a.[ mk_usize 1 ] <: u64) (b.[ mk_usize 4 ] <: u64) <: u128) +!
-          (m (a.[ mk_usize 2 ] <: u64) (b.[ mk_usize 3 ] <: u64) <: u128)
-          <:
-          u128) +!
-        (m (a.[ mk_usize 3 ] <: u64) (b.[ mk_usize 2 ] <: u64) <: u128)
-        <:
-        u128) +!
-      (m (a.[ mk_usize 4 ] <: u64) (b.[ mk_usize 1 ] <: u64) <: u128);
-      ((m (a.[ mk_usize 2 ] <: u64) (b.[ mk_usize 4 ] <: u64) <: u128) +!
-        (m (a.[ mk_usize 3 ] <: u64) (b.[ mk_usize 3 ] <: u64) <: u128)
-        <:
-        u128) +!
-      (m (a.[ mk_usize 4 ] <: u64) (b.[ mk_usize 2 ] <: u64) <: u128);
-      (m (a.[ mk_usize 3 ] <: u64) (b.[ mk_usize 4 ] <: u64) <: u128) +!
-      (m (a.[ mk_usize 4 ] <: u64) (b.[ mk_usize 3 ] <: u64) <: u128);
-      m (a.[ mk_usize 4 ] <: u64) (b.[ mk_usize 4 ] <: u64)
-    ]
-  in
-  FStar.Pervasives.assert_norm (Prims.eq2 (List.Tot.length list) 9);
-  Rust_primitives.Hax.array_of_list 9 list
+assume
+val impl_Scalar52__from_bytes_wide': bytes: t_Array u8 (mk_usize 64) -> t_Scalar52
 
-let impl_Scalar52__montgomery_reduce__part2 (sum: u128) : (u128 & u64) =
-  let w:u64 = (cast (sum <: u128) <: u64) &. ((mk_u64 1 <<! mk_i32 52 <: u64) -! mk_u64 1 <: u64) in
-  sum >>! mk_i32 52, w <: (u128 & u64)
+unfold
+let impl_Scalar52__from_bytes_wide = impl_Scalar52__from_bytes_wide'
+
+assume
+val impl_Scalar52__to_bytes': self: t_Scalar52 -> t_Array u8 (mk_usize 32)
+
+unfold
+let impl_Scalar52__to_bytes = impl_Scalar52__to_bytes'
+
+/// Construct a scalar by reducing a 512-bit little-endian integer modulo ℓ.
+let impl_Scalar__from_bytes_mod_order_wide (bytes: t_Array u8 (mk_usize 64)) : t_Scalar =
+  Scalar (impl_Scalar52__to_bytes (impl_Scalar52__from_bytes_wide bytes <: t_Scalar52)) <: t_Scalar
+
+assume
+val impl_Scalar52__add': a: t_Scalar52 -> b: t_Scalar52 -> t_Scalar52
+
+unfold
+let impl_Scalar52__add = impl_Scalar52__add'
+
+assume
+val impl_Scalar52__sub': a: t_Scalar52 -> b: t_Scalar52 -> t_Scalar52
+
+unfold
+let impl_Scalar52__sub = impl_Scalar52__sub'
+
+assume
+val impl_Scalar52__mul_internal': a: t_Scalar52 -> b: t_Scalar52 -> t_Array u128 (mk_usize 9)
+
+unfold
+let impl_Scalar52__mul_internal = impl_Scalar52__mul_internal'
+
+assume
+val impl_Scalar52__montgomery_reduce': limbs: t_Array u128 (mk_usize 9) -> t_Scalar52
+
+unfold
+let impl_Scalar52__montgomery_reduce = impl_Scalar52__montgomery_reduce'
+
+assume
+val impl_Scalar52__montgomery_mul': a: t_Scalar52 -> b: t_Scalar52 -> t_Scalar52
+
+unfold
+let impl_Scalar52__montgomery_mul = impl_Scalar52__montgomery_mul'
+
+assume
+val impl_Scalar52__montgomery_reduce__part1': sum: u128 -> (u128 & u64)
+
+unfold
+let impl_Scalar52__montgomery_reduce__part1 = impl_Scalar52__montgomery_reduce__part1'
+
+assume
+val impl_Scalar52__montgomery_reduce__part2': sum: u128 -> (u128 & u64)
+
+unfold
+let impl_Scalar52__montgomery_reduce__part2 = impl_Scalar52__montgomery_reduce__part2'
 
 /// `L` is the group order ℓ = 2^252 + 27742317777372353535851937790883648493.
 let v_L: t_Scalar52 =
@@ -386,212 +169,8 @@ let v_L: t_Scalar52 =
   <:
   t_Scalar52
 
-let impl_Scalar52__sub (a b: t_Scalar52) : t_Scalar52 =
-  let difference:t_Scalar52 = impl_Scalar52__ZERO in
-  let mask:u64 = (mk_u64 1 <<! mk_i32 52 <: u64) -! mk_u64 1 in
-  let (borrow: u64):u64 = mk_u64 0 in
-  let (borrow: u64), (difference: t_Scalar52) =
-    Rust_primitives.Hax.Folds.fold_range (mk_usize 0)
-      (mk_usize 5)
-      (fun temp_0_ temp_1_ ->
-          let (borrow: u64), (difference: t_Scalar52) = temp_0_ in
-          let _:usize = temp_1_ in
-          true)
-      (borrow, difference <: (u64 & t_Scalar52))
-      (fun temp_0_ i ->
-          let (borrow: u64), (difference: t_Scalar52) = temp_0_ in
-          let i:usize = i in
-          let borrow:u64 =
-            Core_models.Num.impl_u64__wrapping_sub (a._0.[ i ] <: u64)
-              ((b._0.[ i ] <: u64) +! (borrow >>! mk_i32 63 <: u64) <: u64)
-          in
-          let difference:t_Scalar52 =
-            {
-              difference with
-              _0
-              =
-              Rust_primitives.Hax.Monomorphized_update_at.update_at_usize difference._0
-                i
-                (borrow &. mask <: u64)
-            }
-            <:
-            t_Scalar52
-          in
-          borrow, difference <: (u64 & t_Scalar52))
-  in
-  let underflow:Subtle.t_Choice =
-    Core_models.Convert.f_from #Subtle.t_Choice
-      #u8
-      #FStar.Tactics.Typeclasses.solve
-      (cast (borrow >>! mk_i32 63 <: u64) <: u8)
-  in
-  let (carry: u64):u64 = mk_u64 0 in
-  let (carry: u64), (difference: t_Scalar52) =
-    Rust_primitives.Hax.Folds.fold_range (mk_usize 0)
-      (mk_usize 5)
-      (fun temp_0_ temp_1_ ->
-          let (carry: u64), (difference: t_Scalar52) = temp_0_ in
-          let _:usize = temp_1_ in
-          true)
-      (carry, difference <: (u64 & t_Scalar52))
-      (fun temp_0_ i ->
-          let (carry: u64), (difference: t_Scalar52) = temp_0_ in
-          let i:usize = i in
-          let addend:u64 =
-            Subtle.f_conditional_select #u64
-              #FStar.Tactics.Typeclasses.solve
-              (mk_u64 0)
-              (v_L._0.[ i ] <: u64)
-              underflow
-          in
-          let carry:u64 =
-            ((carry >>! mk_i32 52 <: u64) +! (difference._0.[ i ] <: u64) <: u64) +! addend
-          in
-          let difference:t_Scalar52 =
-            {
-              difference with
-              _0
-              =
-              Rust_primitives.Hax.Monomorphized_update_at.update_at_usize difference._0
-                i
-                (carry &. mask <: u64)
-            }
-            <:
-            t_Scalar52
-          in
-          carry, difference <: (u64 & t_Scalar52))
-  in
-  difference
-
-let impl_Scalar52__add (a b: t_Scalar52) : t_Scalar52 =
-  let sum:t_Scalar52 = impl_Scalar52__ZERO in
-  let mask:u64 = (mk_u64 1 <<! mk_i32 52 <: u64) -! mk_u64 1 in
-  let (carry: u64):u64 = mk_u64 0 in
-  let (carry: u64), (sum: t_Scalar52) =
-    Rust_primitives.Hax.Folds.fold_range (mk_usize 0)
-      (mk_usize 5)
-      (fun temp_0_ temp_1_ ->
-          let (carry: u64), (sum: t_Scalar52) = temp_0_ in
-          let _:usize = temp_1_ in
-          true)
-      (carry, sum <: (u64 & t_Scalar52))
-      (fun temp_0_ i ->
-          let (carry: u64), (sum: t_Scalar52) = temp_0_ in
-          let i:usize = i in
-          let carry:u64 =
-            ((a._0.[ i ] <: u64) +! (b._0.[ i ] <: u64) <: u64) +! (carry >>! mk_i32 52 <: u64)
-          in
-          let sum:t_Scalar52 =
-            {
-              sum with
-              _0
-              =
-              Rust_primitives.Hax.Monomorphized_update_at.update_at_usize sum._0
-                i
-                (carry &. mask <: u64)
-            }
-            <:
-            t_Scalar52
-          in
-          carry, sum <: (u64 & t_Scalar52))
-  in
-  impl_Scalar52__sub sum v_L
-
 /// `L * LFACTOR ≡ -1  (mod 2^52)`.
 let v_LFACTOR: u64 = mk_u64 1439961107955227
-
-let impl_Scalar52__montgomery_reduce__part1 (sum: u128) : (u128 & u64) =
-  let p:u64 =
-    (Core_models.Num.impl_u64__wrapping_mul (cast (sum <: u128) <: u64) v_LFACTOR <: u64) &.
-    ((mk_u64 1 <<! mk_i32 52 <: u64) -! mk_u64 1 <: u64)
-  in
-  (sum +! (m p (v_L._0.[ mk_usize 0 ] <: u64) <: u128) <: u128) >>! mk_i32 52, p <: (u128 & u64)
-
-let impl_Scalar52__montgomery_reduce (limbs: t_Array u128 (mk_usize 9)) : t_Scalar52 =
-  let l:t_Array u64 (mk_usize 5) = v_L._0 in
-  let (carry: u128), (n0: u64) =
-    impl_Scalar52__montgomery_reduce__part1 (limbs.[ mk_usize 0 ] <: u128)
-  in
-  let (carry: u128), (n1: u64) =
-    impl_Scalar52__montgomery_reduce__part1 ((carry +! (limbs.[ mk_usize 1 ] <: u128) <: u128) +!
-        (m n0 (l.[ mk_usize 1 ] <: u64) <: u128)
-        <:
-        u128)
-  in
-  let (carry: u128), (n2: u64) =
-    impl_Scalar52__montgomery_reduce__part1 (((carry +! (limbs.[ mk_usize 2 ] <: u128) <: u128) +!
-          (m n0 (l.[ mk_usize 2 ] <: u64) <: u128)
-          <:
-          u128) +!
-        (m n1 (l.[ mk_usize 1 ] <: u64) <: u128)
-        <:
-        u128)
-  in
-  let (carry: u128), (n3: u64) =
-    impl_Scalar52__montgomery_reduce__part1 (((carry +! (limbs.[ mk_usize 3 ] <: u128) <: u128) +!
-          (m n1 (l.[ mk_usize 2 ] <: u64) <: u128)
-          <:
-          u128) +!
-        (m n2 (l.[ mk_usize 1 ] <: u64) <: u128)
-        <:
-        u128)
-  in
-  let (carry: u128), (n4: u64) =
-    impl_Scalar52__montgomery_reduce__part1 ((((carry +! (limbs.[ mk_usize 4 ] <: u128) <: u128) +!
-            (m n0 (l.[ mk_usize 4 ] <: u64) <: u128)
-            <:
-            u128) +!
-          (m n2 (l.[ mk_usize 2 ] <: u64) <: u128)
-          <:
-          u128) +!
-        (m n3 (l.[ mk_usize 1 ] <: u64) <: u128)
-        <:
-        u128)
-  in
-  let (carry: u128), (r0: u64) =
-    impl_Scalar52__montgomery_reduce__part2 ((((carry +! (limbs.[ mk_usize 5 ] <: u128) <: u128) +!
-            (m n1 (l.[ mk_usize 4 ] <: u64) <: u128)
-            <:
-            u128) +!
-          (m n3 (l.[ mk_usize 2 ] <: u64) <: u128)
-          <:
-          u128) +!
-        (m n4 (l.[ mk_usize 1 ] <: u64) <: u128)
-        <:
-        u128)
-  in
-  let (carry: u128), (r1: u64) =
-    impl_Scalar52__montgomery_reduce__part2 (((carry +! (limbs.[ mk_usize 6 ] <: u128) <: u128) +!
-          (m n2 (l.[ mk_usize 4 ] <: u64) <: u128)
-          <:
-          u128) +!
-        (m n4 (l.[ mk_usize 2 ] <: u64) <: u128)
-        <:
-        u128)
-  in
-  let (carry: u128), (r2: u64) =
-    impl_Scalar52__montgomery_reduce__part2 ((carry +! (limbs.[ mk_usize 7 ] <: u128) <: u128) +!
-        (m n3 (l.[ mk_usize 4 ] <: u64) <: u128)
-        <:
-        u128)
-  in
-  let (carry: u128), (r3: u64) =
-    impl_Scalar52__montgomery_reduce__part2 ((carry +! (limbs.[ mk_usize 8 ] <: u128) <: u128) +!
-        (m n4 (l.[ mk_usize 4 ] <: u64) <: u128)
-        <:
-        u128)
-  in
-  let r4:u64 = cast (carry <: u128) <: u64 in
-  impl_Scalar52__sub (Scalar52
-      (let list = [r0; r1; r2; r3; r4] in
-        FStar.Pervasives.assert_norm (Prims.eq2 (List.Tot.length list) 5);
-        Rust_primitives.Hax.array_of_list 5 list)
-      <:
-      t_Scalar52)
-    v_L
-
-let impl_Scalar52__montgomery_mul (a b: t_Scalar52) : t_Scalar52 =
-  impl_Scalar52__montgomery_reduce (impl_Scalar52__mul_internal a b <: t_Array u128 (mk_usize 9))
 
 /// `R = 2^260 mod ℓ`, the Montgomery modulus.
 let v_R: t_Scalar52 =
@@ -672,126 +251,3 @@ let v_RR: t_Scalar52 =
     Rust_primitives.Hax.array_of_list 5 list)
   <:
   t_Scalar52
-
-let impl_Scalar52__from_bytes_wide (bytes: t_Array u8 (mk_usize 64)) : t_Scalar52 =
-  let words:t_Array u64 (mk_usize 8) = Rust_primitives.Hax.repeat (mk_u64 0) (mk_usize 8) in
-  let words:t_Array u64 (mk_usize 8) =
-    Rust_primitives.Hax.Folds.fold_range (mk_usize 0)
-      (mk_usize 8)
-      (fun words temp_1_ ->
-          let words:t_Array u64 (mk_usize 8) = words in
-          let _:usize = temp_1_ in
-          true)
-      words
-      (fun words i ->
-          let words:t_Array u64 (mk_usize 8) = words in
-          let i:usize = i in
-          Rust_primitives.Hax.Folds.fold_range (mk_usize 0)
-            (mk_usize 8)
-            (fun words temp_1_ ->
-                let words:t_Array u64 (mk_usize 8) = words in
-                let _:usize = temp_1_ in
-                true)
-            words
-            (fun words j ->
-                let words:t_Array u64 (mk_usize 8) = words in
-                let j:usize = j in
-                Rust_primitives.Hax.Monomorphized_update_at.update_at_usize words
-                  i
-                  ((words.[ i ] <: u64) |.
-                    ((cast (bytes.[ (i *! mk_usize 8 <: usize) +! j <: usize ] <: u8) <: u64) <<!
-                      (j *! mk_usize 8 <: usize)
-                      <:
-                      u64)
-                    <:
-                    u64)
-                <:
-                t_Array u64 (mk_usize 8))
-          <:
-          t_Array u64 (mk_usize 8))
-  in
-  let mask:u64 = (mk_u64 1 <<! mk_i32 52 <: u64) -! mk_u64 1 in
-  let lo:t_Scalar52 =
-    Scalar52
-    (let list =
-        [
-          (words.[ mk_usize 0 ] <: u64) &. mask;
-          (((words.[ mk_usize 0 ] <: u64) >>! mk_i32 52 <: u64) |.
-            ((words.[ mk_usize 1 ] <: u64) <<! mk_i32 12 <: u64)
-            <:
-            u64) &.
-          mask;
-          (((words.[ mk_usize 1 ] <: u64) >>! mk_i32 40 <: u64) |.
-            ((words.[ mk_usize 2 ] <: u64) <<! mk_i32 24 <: u64)
-            <:
-            u64) &.
-          mask;
-          (((words.[ mk_usize 2 ] <: u64) >>! mk_i32 28 <: u64) |.
-            ((words.[ mk_usize 3 ] <: u64) <<! mk_i32 36 <: u64)
-            <:
-            u64) &.
-          mask;
-          (((words.[ mk_usize 3 ] <: u64) >>! mk_i32 16 <: u64) |.
-            ((words.[ mk_usize 4 ] <: u64) <<! mk_i32 48 <: u64)
-            <:
-            u64) &.
-          mask
-        ]
-      in
-      FStar.Pervasives.assert_norm (Prims.eq2 (List.Tot.length list) 5);
-      Rust_primitives.Hax.array_of_list 5 list)
-    <:
-    t_Scalar52
-  in
-  let hi:t_Scalar52 =
-    Scalar52
-    (let list =
-        [
-          ((words.[ mk_usize 4 ] <: u64) >>! mk_i32 4 <: u64) &. mask;
-          (((words.[ mk_usize 4 ] <: u64) >>! mk_i32 56 <: u64) |.
-            ((words.[ mk_usize 5 ] <: u64) <<! mk_i32 8 <: u64)
-            <:
-            u64) &.
-          mask;
-          (((words.[ mk_usize 5 ] <: u64) >>! mk_i32 44 <: u64) |.
-            ((words.[ mk_usize 6 ] <: u64) <<! mk_i32 20 <: u64)
-            <:
-            u64) &.
-          mask;
-          (((words.[ mk_usize 6 ] <: u64) >>! mk_i32 32 <: u64) |.
-            ((words.[ mk_usize 7 ] <: u64) <<! mk_i32 32 <: u64)
-            <:
-            u64) &.
-          mask;
-          (words.[ mk_usize 7 ] <: u64) >>! mk_i32 20
-        ]
-      in
-      FStar.Pervasives.assert_norm (Prims.eq2 (List.Tot.length list) 5);
-      Rust_primitives.Hax.array_of_list 5 list)
-    <:
-    t_Scalar52
-  in
-  let lo:t_Scalar52 = impl_Scalar52__montgomery_mul lo v_R in
-  let hi:t_Scalar52 = impl_Scalar52__montgomery_mul hi v_RR in
-  impl_Scalar52__add hi lo
-
-/// Construct a scalar by reducing a 512-bit little-endian integer modulo ℓ.
-let impl_Scalar__from_bytes_mod_order_wide (bytes: t_Array u8 (mk_usize 64)) : t_Scalar =
-  Scalar (impl_Scalar52__to_bytes (impl_Scalar52__from_bytes_wide bytes <: t_Scalar52)) <: t_Scalar
-
-/// Generate a random scalar using the provided RNG.
-let impl_Scalar__random
-      (#v_R: Type0)
-      (#[FStar.Tactics.Typeclasses.tcresolve ()] i0: Rand_core.t_RngCore v_R)
-      (#[FStar.Tactics.Typeclasses.tcresolve ()] i1: Rand_core.t_CryptoRng v_R)
-      (rng: v_R)
-    : (v_R & t_Scalar) =
-  let bytes:t_Array u8 (mk_usize 64) = Rust_primitives.Hax.repeat (mk_u8 0) (mk_usize 64) in
-  let (tmp0: v_R), (tmp1: t_Array u8 (mk_usize 64)) =
-    Rand_core.f_fill_bytes #v_R #FStar.Tactics.Typeclasses.solve rng bytes
-  in
-  let rng:v_R = tmp0 in
-  let bytes:t_Array u8 (mk_usize 64) = tmp1 in
-  let _:Prims.unit = () in
-  let hax_temp_output:t_Scalar = impl_Scalar__from_bytes_mod_order_wide bytes in
-  rng, hax_temp_output <: (v_R & t_Scalar)
